GameCore erweitert

Dafny15Puzzle/GameCore.dfy
@@ -1,1 +1,140 @@
-﻿
+﻿class Game{
+	var borders : array<int>;
+	var items : array<int>;
+
+	constructor Init(a: array<int>)
+	modifies this
+	{
+		borders := new int[8];
+		borders[0] := 0;
+		borders[1] := 3;
+		borders[2] := 4;
+		borders[3] := 7;
+		borders[4] := 8;
+		borders[5] := 11;
+		borders[6] := 12;
+		borders[7] := 15;
+		items := a;
+	}
+
+	predicate Valid()
+	reads this;
+	{
+		items != null && items.Length == 16 && borders != null && borders.Length == 8
+	}
+
+	method FindPosById(id: int) returns (pos: int)
+	requires Valid();
+	ensures old(items) == items;
+	ensures Valid();
+	{
+		var i := 0;
+		while(i <= 15)
+		invariant 0 <= i <= 16;
+		invariant old(items) == items;
+		{
+			if(items[i] == id)
+			{
+				pos := i;
+			}
+			i := i + 1;
+		}
+	}
+
+	method FindEmpty() returns (pos: int)
+	requires Valid();
+	ensures old(items) == items;
+	ensures Valid();
+	{
+		var i := 0;
+		while(i <= 15)
+		invariant 0 <= i <= 16;
+		invariant old(items) == items;
+		{
+			if(items[i] == 15)
+			{
+				pos := i;
+			}
+			i := i + 1;
+		}
+	}
+
+	method GetIdByPos(pos: int) returns (id: int)
+	requires Valid();
+	requires 0 <= pos < items.Length;
+	ensures old(items) == items;
+	ensures Valid();
+	{
+		id := items[pos];
+	}
+
+	method BoardSolved() returns (b: bool)
+	requires Valid();
+	ensures old(items) == items;
+	ensures Valid();
+	{
+		var i := 0;
+		b := true;
+
+		while(i <= 15)
+		{
+			if(items[i] != i)
+			{
+				b := false;
+			}
+			i := i + 1;
+		}
+	}
+
+	method IsSolvable() returns (b: bool)
+	requires Valid();
+	ensures old(items) == items;
+	ensures Valid();
+	{
+		var i := 1;
+		var n := 0;
+		b := false;
+
+		while(i <= 15)
+		{
+			var num1 := GetIdByPos(i);
+			var num2 := GetIdByPos(i - 1);
+
+			if(num1 > num2)
+			{
+				n := n + 1;
+			}
+
+			i := i + 1;
+		}
+
+		var emptyPos := FindEmpty();
+		if(n % 2 == (emptyPos + emptyPos / 4) % 2)
+		{
+			b := true;
+		}
+	}
+
+	method IsBorderSwitch(x: int, y: int) returns (b: bool)
+	requires Valid();
+	ensures old(items) == items;
+	ensures Valid();
+	{
+		b := (BordersContain(x) && BordersContain(y));
+	}
+
+	function method BordersContain(v: int) : bool
+	requires Valid();
+	reads this;
+	reads borders;
+	{
+		exists i :: 0 <= i < borders.Length && borders[i] == v
+	}
+
+	method CanMove(id: int) returns(target: int)
+	requires Valid();
+	ensures Valid();
+	{
+		
+	}
+}
